progs/entailment_tests.v
@@ -1,0 +1,584 @@
+Load loadpath.
+Require Import Coqlib msl.Coqlib2.
+Require Import veric.SeparationLogic.
+Require Import Ctypes.
+Require veric.SequentialClight.
+Import SequentialClight.SeqC.CSL.
+Require Import progs.field_mapsto.
+Require Import progs.client_lemmas.
+Require Import progs.assert_lemmas.
+Require Import progs.list.
+Require Import Clightdefs. 
+Require Import progs.test1. Module P := progs.test1.
+Require Import progs.ilseg.
+
+Local Open Scope logic.
+
+Definition sumlist_spec :=
+ DECLARE P._sumlist
+  WITH sh_contents 
+  PRE [ P._p : t_listptr]  lift2 (ilseg (fst sh_contents) (snd sh_contents)) (eval_id P._p) (lift0 nullval)
+  POST [ tint ]  local (lift1 (eq (Vint (fold_right Int.add Int.zero (snd sh_contents)))) retval).
+
+Definition reverse_spec :=
+ DECLARE P._reverse
+  WITH sh_contents : share * list int
+  PRE  [ P._p : t_listptr ] !! writable_share (fst sh_contents) &&
+        lift2 (ilseg (fst sh_contents) (snd sh_contents)) (eval_id P._p) (lift0 nullval)
+  POST [ t_listptr ] lift2 (ilseg (fst sh_contents) (rev (snd sh_contents))) retval (lift0 nullval).
+
+Definition main_spec :=
+ DECLARE P._main
+  WITH u : unit
+  PRE  [] main_pre P.prog u
+  POST [ tint ] main_post P.prog u.
+
+Definition main_spec' := (P._main, mk_funspec (nil, tint) _ (main_pre P.prog) (main_post P.prog)).
+
+Definition Vprog : varspecs := (P._three, Tarray P.t_struct_list 3 noattr)::nil.
+
+Definition Gprog : funspecs := 
+    sumlist_spec :: reverse_spec :: main_spec::nil.
+
+Definition Gtot := do_builtins (prog_defs P.prog) ++ Gprog.
+
+Lemma et_1:
+ forall (sh: share) (contents: list int),
+    let Delta := func_tycontext P.f_sumlist Vprog Gtot  in
+PROP  ()
+LOCAL 
+(tc_environ
+   (update_tycon
+      (update_tycon Delta (Sset P._s (Econst_int (Int.repr 0) tint)))
+      (Sset P._t (Etempvar P._p (tptr P.t_struct_list))));
+lift2 eq (eval_id P._t) (eval_expr (Etempvar P._p (tptr P.t_struct_list)));
+lift2 eq (eval_id P._s) (eval_expr (Econst_int (Int.repr 0) tint));
+tc_formals ((P._p, tptr P.t_struct_list) :: nil))
+SEP  (lift2 (ilseg sh contents) (eval_id P._p) (lift0 nullval)*
+stackframe_of P.f_sumlist)
+|-- PROP  ()
+    LOCAL 
+    (lift1
+       (fun v : val =>
+        fold_right Int.add Int.zero contents =
+        Int.add (force_int v) (fold_right Int.add Int.zero contents))
+       (eval_id P._s))
+    SEP  (TT * lift2 (ilseg sh contents) (eval_id P._t) (lift0 nullval)).
+Proof.  intros.
+ go_lower.
+ varname P._t _t.
+ varname P._p _p.
+ varname P._s _s.
+ findvars.
+ subst.
+ rewrite Int.add_zero_l; normalize; rewrite sepcon_comm; apply sepcon_TT.
+Qed.
+
+Definition partial_sum (contents cts: list int) (v: val) := 
+     fold_right Int.add Int.zero contents = Int.add (force_int  v) (fold_right Int.add Int.zero cts).
+
+Lemma et_2: forall (sh: share) (contents: list int),
+    let Delta := func_tycontext P.f_sumlist Vprog Gtot  in
+EX  cts : list int,
+PROP  ()
+LOCAL  (lift1 (partial_sum contents cts) (eval_id P._s))
+SEP  (TT * lift2 (ilseg sh cts) (eval_id P._t) (lift0 nullval))
+  |-- local
+      (tc_expr
+         (update_tycon
+            (update_tycon Delta (Sset P._s (Econst_int (Int.repr 0) tint)))
+            (Sset P._t (Etempvar P._p (tptr P.t_struct_list))))
+         (Etempvar P._t (tptr P.t_struct_list))).
+Proof. intros.
+ intro; apply TT_right.
+Qed.
+
+Lemma et_3: forall (sh: share) (contents: list int),
+    let Delta := func_tycontext P.f_sumlist Vprog Gtot  in
+
+local
+  (lift1 (typed_false (typeof (Etempvar P._t (tptr P.t_struct_list))))
+     (eval_expr (Etempvar P._t (tptr P.t_struct_list)))) &&
+(EX  cts : list int,
+ PROP  ()
+ LOCAL 
+ (lift1
+    (fun v : val =>
+     fold_right Int.add Int.zero contents =
+     Int.add (force_int v) (fold_right Int.add Int.zero cts)) (eval_id P._s))
+   SEP  (TT * lift2 (ilseg sh cts) (eval_id P._t) (lift0 nullval)))
+|-- overridePost
+      (PROP  ()
+       LOCAL 
+       (lift1
+          (fun v : val => fold_right Int.add Int.zero contents = force_int v)
+          (eval_id P._s))  SEP  (TT))
+      (frame_ret_assert
+         (function_body_ret_assert tint
+            (local
+               (lift1 (eq (Vint (fold_right Int.add Int.zero contents)))
+                  retval))) (stackframe_of P.f_sumlist)) EK_normal None.
+Proof. intros.
+normalize. go_lower.
+  rewrite H, H0. normalize.
+Qed.
+
+Lemma et_4: forall (sh: share) (contents: list int),
+    let Delta := func_tycontext P.f_sumlist Vprog Gtot  in
+forall (cts : list int),
+local
+  (tc_environ
+     (update_tycon
+        (update_tycon Delta (Sset P._s (Econst_int (Int.repr 0) tint)))
+        (Sset P._t (Etempvar P._p (tptr P.t_struct_list))))) &&
+PROP  ()
+LOCAL 
+(lift1 (typed_true (typeof (Etempvar P._t (tptr P.t_struct_list))))
+   (eval_id P._t); lift1 (partial_sum contents cts) (eval_id P._s))
+SEP  (TT * lift2 (ilseg sh cts) (eval_id P._t) (lift0 nullval))
+|-- PROP  ()
+    LOCAL 
+    (lift1 (typed_true (typeof (Etempvar P._t (tptr P.t_struct_list))))
+       (eval_id P._t); lift1 (partial_sum contents cts) (eval_id P._s))
+    SEP  (TT * lift2 (ilseg_cons sh cts) (eval_id P._t) (lift0 nullval)).
+Proof. intros.
+normalize; go_lower; rewrite ilseg_nonnull; normalize.
+Qed.
+
+Lemma et_5: forall (sh: share) (contents: list int),
+    let Delta := func_tycontext P.f_sumlist Vprog Gtot  in
+ forall (h: int) (r: list int) (y: val) (old_t: val) (x: val),
+PROP  ()
+LOCAL 
+(tc_environ
+   (exit_tycon
+      (Sset P._s (Ebinop Oadd (Etempvar P._s tint) (Etempvar P._h tint) tint))
+      (initialized P._t
+         (initialized P._h (initialized P._t (initialized P._s Delta))))
+      EK_normal);
+lift2 eq (eval_id P._s)
+  (lift2
+     (eval_binop Oadd (typeof (Etempvar P._s tint))
+        (typeof (Etempvar P._h tint))) (lift0 x) (eval_id P._h));
+lift2 eq (eval_id P._t) (lift0 y); lift2 eq (eval_id P._h) (lift0 (Vint h));
+lift2 ptr_neq (lift0 old_t) (lift0 nullval);
+lift0 (typed_true (typeof (Etempvar P._t (tptr P.t_struct_list))) old_t);
+lift0
+  (fold_right Int.add Int.zero contents =
+   Int.add (force_int x) (fold_right Int.add Int.zero (h :: r))))
+SEP  (lift2 (field_mapsto sh P.t_struct_list P._t) (lift0 old_t) (lift0 y)*
+lift2 (field_mapsto sh P.t_struct_list P._h) (lift0 old_t) (lift0 (Vint h))*
+lift2 (ilseg sh r) (lift0 y) (lift0 nullval)* TT)
+|-- PROP  ()
+    LOCAL 
+    (lift1
+       (fun v : val =>
+        fold_right Int.add Int.zero contents =
+        Int.add (force_int v) (fold_right Int.add Int.zero r)) (eval_id P._s))
+      SEP  (TT * lift2 (ilseg sh r) (eval_id P._t) (lift0 nullval)).
+Proof. intros.
+go_lower.
+varname P._s _s.
+varname P._t  _t.
+varname P._h _h.
+findvars.
+subst. rewrite H5; clear H5.
+destruct (tc_val_extract_int _ _ _ _ H6) as [n H5].
+rewrite H5 in *.
+simpl.
+destruct x; inv H5.
+simpl.
+rewrite (Int.add_assoc i h). normalize.
+rewrite <- (sepcon_comm TT).
+repeat rewrite <- sepcon_assoc.
+apply sepcon_derives; auto.
+normalize.
+Qed.
+
+Lemma et_6: forall (sh: share) (contents: list int),
+    let Delta := func_tycontext P.f_sumlist Vprog Gtot  in
+
+local
+  (tc_environ
+     (update_tycon
+        (update_tycon
+           (update_tycon Delta (Sset P._s (Econst_int (Int.repr 0) tint)))
+           (Sset P._t (Etempvar P._p (tptr P.t_struct_list))))
+        (Swhile (Etempvar P._t (tptr P.t_struct_list))
+           (Ssequence
+              (Sset P._h
+                 (Efield
+                    (Ederef (Etempvar P._t (tptr P.t_struct_list))
+                       P.t_struct_list) P._h tint))
+              (Ssequence
+                 (Sset P._t
+                    (Efield
+                       (Ederef (Etempvar P._t (tptr P.t_struct_list))
+                          P.t_struct_list) P._t (tptr P.t_struct_list)))
+                 (Sset P._s
+                    (Ebinop Oadd (Etempvar P._s tint) (Etempvar P._h tint)
+                       tint))))))) &&
+PROP  ()
+LOCAL 
+(lift1 (fun v : val => fold_right Int.add Int.zero contents = force_int v)
+   (eval_id P._s))  SEP  (TT)
+|-- tc_expropt
+      (update_tycon
+         (update_tycon
+            (update_tycon Delta (Sset P._s (Econst_int (Int.repr 0) tint)))
+            (Sset P._t (Etempvar P._p (tptr P.t_struct_list))))
+         (Swhile (Etempvar P._t (tptr P.t_struct_list))
+            (Ssequence
+               (Sset P._h
+                  (Efield
+                     (Ederef (Etempvar P._t (tptr P.t_struct_list))
+                        P.t_struct_list) P._h tint))
+               (Ssequence
+                  (Sset P._t
+                     (Efield
+                        (Ederef (Etempvar P._t (tptr P.t_struct_list))
+                           P.t_struct_list) P._t (tptr P.t_struct_list)))
+                  (Sset P._s
+                     (Ebinop Oadd (Etempvar P._s tint) (Etempvar P._h tint)
+                        tint)))))) (Some (Etempvar P._s tint))
+      (ret_type
+         (update_tycon
+            (update_tycon
+               (update_tycon Delta (Sset P._s (Econst_int (Int.repr 0) tint)))
+               (Sset P._t (Etempvar P._p (tptr P.t_struct_list))))
+            (Swhile (Etempvar P._t (tptr P.t_struct_list))
+               (Ssequence
+                  (Sset P._h
+                     (Efield
+                        (Ederef (Etempvar P._t (tptr P.t_struct_list))
+                           P.t_struct_list) P._h tint))
+                  (Ssequence
+                     (Sset P._t
+                        (Efield
+                           (Ederef (Etempvar P._t (tptr P.t_struct_list))
+                              P.t_struct_list) P._t (tptr P.t_struct_list)))
+                     (Sset P._s
+                        (Ebinop Oadd (Etempvar P._s tint)
+                           (Etempvar P._h tint) tint))))))) &&
+    lift2
+      (frame_ret_assert
+         (function_body_ret_assert tint
+            (local
+               (lift1 (eq (Vint (fold_right Int.add Int.zero contents)))
+                  retval))) (stackframe_of P.f_sumlist) EK_return)
+      (cast_expropt (Some (Etempvar P._s tint))
+         (ret_type
+            (update_tycon
+               (update_tycon
+                  (update_tycon Delta
+                     (Sset P._s (Econst_int (Int.repr 0) tint)))
+                  (Sset P._t (Etempvar P._p (tptr P.t_struct_list))))
+               (Swhile (Etempvar P._t (tptr P.t_struct_list))
+                  (Ssequence
+                     (Sset P._h
+                        (Efield
+                           (Ederef (Etempvar P._t (tptr P.t_struct_list))
+                              P.t_struct_list) P._h tint))
+                     (Ssequence
+                        (Sset P._t
+                           (Efield
+                              (Ederef (Etempvar P._t (tptr P.t_struct_list))
+                                 P.t_struct_list) P._t (tptr P.t_struct_list)))
+                        (Sset P._s
+                           (Ebinop Oadd (Etempvar P._s tint)
+                              (Etempvar P._h tint) tint)))))))) id.
+Proof. intros.
+normalize.
+go_lower.
+varname P._s _s.
+findvars.
+repeat apply andp_right; normalize.
+rewrite H0.
+unfold tint; rewrite eval_cast_int by auto.
+apply andp_right; apply prop_right.
+auto.
+destruct _s; inv H1; auto.
+Qed.
+
+Lemma et_7: forall (sh: share) (contents: list int),
+    let Delta := func_tycontext P.f_reverse Vprog Gtot in
+ PROP  ()
+LOCAL 
+(tc_environ
+   (update_tycon
+      (update_tycon Delta
+         (Sset P._w (Ecast (Econst_int (Int.repr 0) tint) (tptr tvoid))))
+      (Sset P._v (Etempvar P._p (tptr P.t_struct_list))));
+lift2 eq (eval_id P._v) (eval_expr (Etempvar P._p (tptr P.t_struct_list)));
+lift2 eq (eval_id P._w)
+  (eval_expr (Ecast (Econst_int (Int.repr 0) tint) (tptr tvoid)));
+lift2 and (lift1 (tc_val (tptr P.t_struct_list)) (eval_id P._p)) (lift0 True))
+
+SEP  (lift2 (ilseg sh contents) (eval_id P._p) (lift0 nullval)*
+stackframe_of P.f_reverse)
+|-- PROP  (contents = rev nil ++ contents)
+    LOCAL ()
+    SEP 
+    (lift2 (ilseg sh nil) (eval_id P._w) (lift0 nullval) *
+     lift2 (ilseg sh contents) (eval_id P._v) (lift0 nullval)).
+Proof. intros.
+go_lower.
+varname P._p _p.
+varname P._v _v.
+varname P._w _w.
+findvars.
+subst. simpl; normalize.
+Qed.
+
+Lemma et_8: forall (sh: share) (contents: list int),
+    let Delta := func_tycontext P.f_reverse Vprog Gtot in
+EX  cts1 : list int,
+(EX  cts2 : list int,
+ PROP  (contents = rev cts1 ++ cts2)
+ LOCAL ()
+ SEP 
+ (lift2 (ilseg sh cts1) (eval_id P._w) (lift0 nullval) *
+  lift2 (ilseg sh cts2) (eval_id P._v) (lift0 nullval)))
+|-- local
+      (tc_expr
+         (update_tycon
+            (update_tycon Delta
+               (Sset P._w (Ecast (Econst_int (Int.repr 0) tint) (tptr tvoid))))
+            (Sset P._v (Etempvar P._p (tptr P.t_struct_list))))
+         (Etempvar P._v (tptr P.t_struct_list))).
+Proof.
+intros.
+normalize.
+intros.
+go_lower. apply prop_right; repeat split.
+Qed.
+
+Lemma et_9: forall (sh: share) (contents: list int),
+    let Delta := func_tycontext P.f_reverse Vprog Gtot in
+  forall (cts1 cts2 : list int),
+PROP  (contents = rev cts1 ++ cts2)
+LOCAL 
+(lift1 (typed_false (typeof (Etempvar P._v (tptr P.t_struct_list))))
+   (eval_id P._v))
+SEP 
+(lift2 (ilseg sh cts1) (eval_id P._w) (lift0 nullval) *
+ lift2 (ilseg sh cts2) (eval_id P._v) (lift0 nullval))
+|-- PROP  ()
+    LOCAL ()
+    SEP  (lift2 (ilseg sh (rev contents)) (eval_id P._w) (lift0 nullval)).
+Proof. intros.
+go_lower.
+varname P._w _w. varname P._v _v.
+rewrite H0. normalize. subst.
+rewrite <- app_nil_end. rewrite rev_involutive. auto.
+Qed.
+
+Lemma et_12: forall (sh: share) (contents: list int),
+    let Delta := func_tycontext P.f_reverse Vprog Gtot in
+  forall (cts cts2 : list int),
+local
+  (tc_environ
+     (update_tycon
+        (update_tycon Delta
+           (Sset P._w (Ecast (Econst_int (Int.repr 0) tint) (tptr tvoid))))
+        (Sset P._v (Etempvar P._p (tptr P.t_struct_list))))) &&
+PROP  ()
+LOCAL 
+(lift1 (typed_true (typeof (Etempvar P._v (tptr P.t_struct_list))))
+   (eval_id P._v))
+SEP  (lift2 (ilseg sh cts) (eval_id P._w) (lift0 nullval)*
+lift2 (ilseg sh cts2) (eval_id P._v) (lift0 nullval))
+|-- PROP  ()
+    LOCAL 
+    (lift1 (typed_true (typeof (Etempvar P._v (tptr P.t_struct_list))))
+       (eval_id P._v))
+    SEP  (lift2 (ilseg sh cts) (eval_id P._w) (lift0 nullval)*
+    lift2 (ilseg_cons sh cts2) (eval_id P._v) (lift0 nullval)).
+Proof. intros.
+normalize. 
+go_lower.
+rewrite (ilseg_nonnull sh cts2) by auto.
+normalize.
+Qed.
+
+Lemma et_10: forall (sh: share) (contents: list int),
+    let Delta := func_tycontext P.f_reverse Vprog Gtot in
+  forall (cts : list int) (h : int) (r : list int) (y : val) (old_w : val) (x : val),
+PROP  ()
+LOCAL 
+(tc_environ
+   (exit_tycon (Sset P._v (Etempvar P._t (tptr P.t_struct_list)))
+      (update_tycon
+         (update_tycon
+            (initialized P._t (initialized P._v (initialized P._w Delta)))
+            (Sassign
+               (Efield
+                  (Ederef (Etempvar P._v (tptr P.t_struct_list))
+                     P.t_struct_list) P._t (tptr P.t_struct_list))
+               (Etempvar P._w (tptr P.t_struct_list))))
+         (Sset P._w (Etempvar P._v (tptr P.t_struct_list)))) EK_normal);
+lift2 eq (eval_id P._v) (eval_id P._t); lift2 eq (eval_id P._w) (lift0 x);
+lift2 eq (eval_id P._t) (lift0 y); lift2 ptr_neq (lift0 x) (lift0 nullval);
+lift0 (typed_true (typeof (Etempvar P._v (tptr P.t_struct_list))) x))
+SEP 
+(lift2 (field_mapsto sh P.t_struct_list P._t) (lift0 x)
+   (lift0
+      (eval_cast (typeof (Etempvar P._w (tptr P.t_struct_list)))
+         (tptr P.t_struct_list) old_w))*
+lift2 (field_mapsto sh list_struct P._h) (lift0 x) (lift0 (Vint h))*
+lift2 (ilseg sh r) (lift0 y) (lift0 nullval)*
+lift2 (ilseg sh cts) (lift0 old_w) (lift0 nullval))
+|-- PROP  (rev cts ++ h :: r = rev (h :: cts) ++ r)
+    LOCAL ()
+    SEP 
+    (lift2 (ilseg sh (h :: cts)) (eval_id P._w) (lift0 nullval) *
+     lift2 (ilseg sh r) (eval_id P._v) (lift0 nullval)).
+Proof. intros.
+
+go_lower.
+varname P._w _w.
+varname P._v _v.
+varname P._t _t.
+findvars.
+subst x y _t.
+ normalize. rewrite app_ass. normalize.
+rewrite (ilseg_unroll sh (h::cts)).
+apply derives_trans with (ilseg_cons sh (h :: cts) _w nullval *
+    ilseg sh r _v nullval).
+unfold ilseg_cons, lseg_cons.
+normalize. apply exp_right with (Vint h).
+normalize. apply exp_right with (map Vint cts).
+normalize. apply exp_right with old_w.
+normalize. 
+simpl list_data; simpl list_link.
+erewrite (field_mapsto_typecheck_val _ _ _ _ _ P._struct_list _  noattr); [ | reflexivity].
+type_of_field_tac.
+normalize.
+assert (eval_cast (tptr P.t_struct_list)(tptr P.t_struct_list) old_w = old_w)
+  by (destruct old_w ; inv H; simpl; auto).
+rewrite H0 in *.
+normalize.
+repeat pull_right (field_mapsto sh list_struct P._t _w old_w).
+apply sepcon_derives; auto.
+repeat pull_right (field_mapsto sh list_struct P._h _w (Vint h)).
+apply sepcon_derives; auto.
+rewrite sepcon_comm.
+apply sepcon_derives; auto.
+apply now_later.
+apply sepcon_derives; auto.
+apply orp_right2; auto.
+Qed.
+
+
+Lemma et_11: forall (sh: share) (contents: list int),
+    let Delta := func_tycontext P.f_reverse Vprog Gtot in
+
+local
+  (tc_environ
+     (update_tycon
+        (update_tycon
+           (update_tycon Delta
+              (Sset P._w (Ecast (Econst_int (Int.repr 0) tint) (tptr tvoid))))
+           (Sset P._v (Etempvar P._p (tptr P.t_struct_list))))
+        (Swhile (Etempvar P._v (tptr P.t_struct_list))
+           (Ssequence
+              (Sset P._t
+                 (Efield
+                    (Ederef (Etempvar P._v (tptr P.t_struct_list))
+                       P.t_struct_list) P._t (tptr P.t_struct_list)))
+              (Ssequence
+                 (Sassign
+                    (Efield
+                       (Ederef (Etempvar P._v (tptr P.t_struct_list))
+                          P.t_struct_list) P._t (tptr P.t_struct_list))
+                    (Etempvar P._w (tptr P.t_struct_list)))
+                 (Ssequence
+                    (Sset P._w (Etempvar P._v (tptr P.t_struct_list)))
+                    (Sset P._v (Etempvar P._t (tptr P.t_struct_list))))))))) &&
+PROP  ()
+LOCAL ()
+SEP  (lift2 (ilseg sh (rev contents)) (eval_id P._w) (lift0 nullval))
+|-- tc_expropt
+      (update_tycon
+         (update_tycon
+            (update_tycon Delta
+               (Sset P._w (Ecast (Econst_int (Int.repr 0) tint) (tptr tvoid))))
+            (Sset P._v (Etempvar P._p (tptr P.t_struct_list))))
+         (Swhile (Etempvar P._v (tptr P.t_struct_list))
+            (Ssequence
+               (Sset P._t
+                  (Efield
+                     (Ederef (Etempvar P._v (tptr P.t_struct_list))
+                        P.t_struct_list) P._t (tptr P.t_struct_list)))
+               (Ssequence
+                  (Sassign
+                     (Efield
+                        (Ederef (Etempvar P._v (tptr P.t_struct_list))
+                           P.t_struct_list) P._t (tptr P.t_struct_list))
+                     (Etempvar P._w (tptr P.t_struct_list)))
+                  (Ssequence
+                     (Sset P._w (Etempvar P._v (tptr P.t_struct_list)))
+                     (Sset P._v (Etempvar P._t (tptr P.t_struct_list))))))))
+      (Some (Etempvar P._w (tptr P.t_struct_list)))
+      (ret_type
+         (update_tycon
+            (update_tycon
+               (update_tycon Delta
+                  (Sset P._w
+                     (Ecast (Econst_int (Int.repr 0) tint) (tptr tvoid))))
+               (Sset P._v (Etempvar P._p (tptr P.t_struct_list))))
+            (Swhile (Etempvar P._v (tptr P.t_struct_list))
+               (Ssequence
+                  (Sset P._t
+                     (Efield
+                        (Ederef (Etempvar P._v (tptr P.t_struct_list))
+                           P.t_struct_list) P._t (tptr P.t_struct_list)))
+                  (Ssequence
+                     (Sassign
+                        (Efield
+                           (Ederef (Etempvar P._v (tptr P.t_struct_list))
+                              P.t_struct_list) P._t (tptr P.t_struct_list))
+                        (Etempvar P._w (tptr P.t_struct_list)))
+                     (Ssequence
+                        (Sset P._w (Etempvar P._v (tptr P.t_struct_list)))
+                        (Sset P._v (Etempvar P._t (tptr P.t_struct_list))))))))) &&
+    lift2
+      (frame_ret_assert
+         (function_body_ret_assert (tptr P.t_struct_list)
+            (lift2 (ilseg sh (rev contents)) retval (lift0 nullval)))
+         (stackframe_of P.f_reverse) EK_return)
+      (cast_expropt (Some (Etempvar P._w (tptr P.t_struct_list)))
+         (ret_type
+            (update_tycon
+               (update_tycon
+                  (update_tycon Delta
+                     (Sset P._w
+                        (Ecast (Econst_int (Int.repr 0) tint) (tptr tvoid))))
+                  (Sset P._v (Etempvar P._p (tptr P.t_struct_list))))
+               (Swhile (Etempvar P._v (tptr P.t_struct_list))
+                  (Ssequence
+                     (Sset P._t
+                        (Efield
+                           (Ederef (Etempvar P._v (tptr P.t_struct_list))
+                              P.t_struct_list) P._t (tptr P.t_struct_list)))
+                     (Ssequence
+                        (Sassign
+                           (Efield
+                              (Ederef (Etempvar P._v (tptr P.t_struct_list))
+                                 P.t_struct_list) P._t (tptr P.t_struct_list))
+                           (Etempvar P._w (tptr P.t_struct_list)))
+                        (Ssequence
+                           (Sset P._w (Etempvar P._v (tptr P.t_struct_list)))
+                           (Sset P._v (Etempvar P._t (tptr P.t_struct_list))))))))))
+      id.
+Proof. intros.
+normalize.
+go_lower.
+varname P._w _w.
+findvars.
+normalize.
+apply andp_right.
+apply prop_right; repeat split.
+erewrite eval_cast_pointer2; try eassumption; simpl; reflexivity.
+erewrite eval_cast_pointer2; try eassumption; simpl; auto; reflexivity.
+Qed.
