progs/ilseg.v
@@ -1,0 +1,121 @@
+Load loadpath.
+Require Import Coqlib msl.Coqlib2.
+Require Import veric.SeparationLogic.
+Require Import Ctypes.
+Require veric.SequentialClight.
+Import SequentialClight.SeqC.CSL.
+Require Import progs.field_mapsto.
+Require Import progs.assert_lemmas.
+Require Import progs.client_lemmas.
+Require Import progs.list.
+Require Import Clightdefs.
+Require  progs.test1.  Module P := progs.test1.
+Local Open Scope logic.
+
+Definition t_listptr := tptr P.t_struct_list.
+
+Instance t_list_spec: listspec t_listptr.
+Proof.
+econstructor.
+reflexivity.
+intro Hx; inv Hx.
+intros.
+unfold unroll_composite; simpl.
+reflexivity.
+econstructor; simpl; reflexivity.
+Defined.
+
+Definition ilseg (sh: share) (s: list int) := lseg t_listptr sh (map Vint s).
+
+Definition ilseg_nil (l: list  int) x z : mpred := !! (ptr_eq x z) && !! (l=nil) && emp.
+Definition ilseg_cons (sh: share) (s: list int) := lseg_cons t_listptr sh (map Vint s).
+
+Lemma ilseg_unroll: forall sh l x z , 
+    ilseg sh l x z = ilseg_nil l x z || ilseg_cons sh l x z.
+Proof.
+intros.
+unfold ilseg at 1.
+rewrite lseg_unroll.
+unfold ilseg_cons, ilseg_nil, ilseg.
+f_equal.
+f_equal. f_equal.
+f_equal.
+apply prop_ext; split; intro; destruct l; simpl in *; congruence.
+Qed.
+
+Lemma ilseg_eq: forall sh s p, 
+   typecheck_val p t_listptr = true -> 
+    (ilseg sh s p p = !!(s=nil) && emp).
+Proof. intros. unfold ilseg. rewrite lseg_eq; auto. f_equal. f_equal.
+ apply prop_ext. destruct s; simpl; intuition congruence.
+Qed.
+Hint Rewrite ilseg_eq : normalize.
+
+Lemma ilseg_nonnull:
+  forall sh s v,
+      typed_true t_listptr v ->
+     ilseg sh s v nullval = ilseg_cons sh s v nullval.
+Proof.
+intros. subst. 
+rewrite ilseg_unroll.
+unfold ilseg_cons, ilseg_nil.
+apply pred_ext; normalize.
+apply orp_left; auto. normalize.
+unfold typed_true, strict_bool_val,ptr_eq in *.
+destruct v; simpl in *; try contradiction.
+rewrite H0 in H. inv H.
+intros.
+normalize.
+apply orp_right2.
+assert (~ ptr_eq v nullval).
+intro. unfold typed_true,ptr_eq in *. destruct v; simpl in *; auto.
+rewrite H0 in H; inv H.
+normalize.
+Qed.
+
+Lemma ilseg_nil_eq: forall sh p q, ilseg sh nil p q = !! (ptr_eq p q) && emp.
+Proof. intros.
+ rewrite ilseg_unroll.
+ apply pred_ext.
+ apply orp_left.
+ unfold ilseg_nil.  normalize.
+ unfold ilseg_cons. normalize. unfold lseg_cons. normalize. intros. inv H0.
+ apply orp_right1. unfold ilseg_nil. normalize.
+Qed.
+Hint Rewrite ilseg_nil_eq : normalize.
+
+Lemma lift2_ilseg_cons: 
+ forall sh s p q, lift2 (ilseg_cons sh s)  p q =
+    EX hry:(int * list int * val),
+      match hry with (h,r,y) =>
+       !! (s = h::r) &&
+       (local (lift2 ptr_neq p q) &&
+       (lift2 (field_mapsto sh list_struct list_data) p (lift0 (Vint h)) *
+        lift2 (field_mapsto sh list_struct list_link) p (lift0 y) *
+        |> lift2 (ilseg sh r) (lift0 y) q))
+     end.
+Proof.
+ intros.
+ unfold ilseg_cons, lseg_cons, lift2. extensionality rho. simpl.
+ unfold local, lift1. unfold ptr_neq.
+ unfold ilseg.
+ apply pred_ext; normalize.
+ destruct s; symmetry in H0; inv H0.
+ apply exp_right with (i, s, y). normalize.
+ destruct h as [[h r] y]. normalize.
+ apply exp_right with (Vint h). normalize. apply exp_right with (map Vint r).
+ normalize. apply exp_right with y. normalize.
+ apply andp_right.
+ forget (field_mapsto sh list_struct P._h (p rho) (Vint h) ) as A.
+ forget (|>lseg t_listptr sh (map Vint r) y (q rho)) as B.
+ erewrite (field_mapsto_typecheck_val); try reflexivity.
+ normalize.
+ apply prop_right.
+ replace t_listptr with (type_of_field
+         (unroll_composite_fields list_structid list_struct
+            (Fcons list_data list_dtype
+               (Fcons list_link (Tcomp_ptr list_structid noattr) Fnil)))
+         P._t); auto.
+ type_of_field_tac.
+ normalize.
+Qed.
